Rewrite parser to simpl well-foundedness
The parser no longer needs to assume anything about well-founded
relations on strings or lists of nonterminals; it carries around its own
fuel (which, for correctness, must line up with the length of the string
being parsed, and an upper bound on the list of valid nonterminals).

This means that the parser no longer needs to know anything about the
proofy bits of the string-like type.  With some extra contortions, we
can show that having extra proofy bits doesn't change the behavior of
the parser, and thus that we are free to use the correctness proofs that
come from the string carrying around its proofy bits with it, and the
parser that comes from the string not carrying around any proofy bits.
Not requiring the proofy bits speeds up the (ab)* grammar from around 15
seconds to around 2 seconds, and speeds up the parenthesized numbers
grammar from around 30 minutes to just over a minute!

src/Parsers/BaseTypes.v
@@ -1,5 +1,5 @@
 (** * Definition of the common part of the interface of the CFG parser *)
-Require Import Coq.Lists.List Coq.Init.Wf Coq.Strings.String.
+Require Import Coq.Lists.List Coq.Arith.Wf_nat Coq.Init.Wf Coq.Strings.String.
 Require Import ADTSynthesis.Parsers.ContextFreeGrammar.
 
 Set Implicit Arguments.
@@ -14,16 +14,21 @@ Section recursive_descent_parser.
   Class parser_computational_predataT :=
     { nonterminals_listT : Type;
       initial_nonterminals_data : nonterminals_listT;
+      nonterminals_length : nonterminals_listT -> nat;
       is_valid_nonterminal : nonterminals_listT -> String.string -> bool;
-      remove_nonterminal : nonterminals_listT -> String.string -> nonterminals_listT;
-      nonterminals_listT_R : nonterminals_listT -> nonterminals_listT -> Prop;
+      remove_nonterminal : nonterminals_listT -> String.string -> nonterminals_listT }.
+
+  Class parser_removal_dataT' `{predata : parser_computational_predataT} :=
+    { nonterminals_listT_R : nonterminals_listT -> nonterminals_listT -> Prop
+      := ltof _ nonterminals_length;
       remove_nonterminal_dec : forall ls nonterminal,
                                  is_valid_nonterminal ls nonterminal
                                  -> nonterminals_listT_R (remove_nonterminal ls nonterminal) ls;
-      ntl_wf : well_founded nonterminals_listT_R }.
-
-  Class parser_removal_dataT' `{predata : parser_computational_predataT} :=
-    { remove_nonterminal_1
+      remove_nonterminal_noninc : forall ls nonterminal,
+                                    ~nonterminals_listT_R ls (remove_nonterminal ls nonterminal);
+      ntl_wf : well_founded nonterminals_listT_R
+      := well_founded_ltof _ _;
+      remove_nonterminal_1
       : forall ls ps ps',
           is_valid_nonterminal (remove_nonterminal ls ps) ps'
           -> is_valid_nonterminal ls ps';
@@ -31,4 +36,11 @@ Section recursive_descent_parser.
       : forall ls ps ps',
           is_valid_nonterminal (remove_nonterminal ls ps) ps' = false
           <-> is_valid_nonterminal ls ps' = false \/ ps = ps' }.
+
+  Class boolean_parser_dataT :=
+    { predata :> parser_computational_predataT;
+      split_string_for_production
+      : item Char -> production Char -> String -> list nat }.
+
+  Global Coercion predata : boolean_parser_dataT >-> parser_computational_predataT.
 End recursive_descent_parser.
