src/Parsers/BooleanRecognizer.v
@@ -3,7 +3,7 @@ Require Import Coq.Lists.List.
 Require Import Coq.Arith.EqNat.
 Require Import Coq.Arith.Compare_dec Coq.Arith.Wf_nat.
 Require Import ADTSynthesis.Parsers.ContextFreeGrammar.
-Require Import ADTSynthesis.Parsers.BaseTypes ADTSynthesis.Parsers.BooleanBaseTypes.
+Require Import ADTSynthesis.Parsers.BaseTypes.
 Require Import ADTSynthesis.Parsers.StringLike.Properties.
 Require Import ADTSynthesis.Common ADTSynthesis.Common.Wf.
 
@@ -11,7 +11,7 @@ Set Implicit Arguments.
 Local Open Scope string_like_scope.
 
 Section recursive_descent_parser.
-  Context {Char} {HSL : StringLike Char} {HSLP : StringLikeProperties Char} {G : grammar Char}.
+  Context {Char} {HSL : StringLike Char} {G : grammar Char}.
   Context {data : @boolean_parser_dataT Char _}.
 
   Section bool.
@@ -27,10 +27,10 @@ Section recursive_descent_parser.
            end.
 
       Section production.
-        Context {str0}
+        Context {len0}
                 (parse_nonterminal
-                 : forall (str : String),
-                     str ≤s str0
+                 : forall (str : String) (len : nat),
+                     len <= len0
                      -> String.string
                      -> bool).
 
@@ -38,7 +38,8 @@ Section recursive_descent_parser.
             But we may do so on any particular split. *)
         Fixpoint parse_production
                  (str : String)
-                 (pf : str ≤s str0)
+                 (len : nat)
+                 (pf : len <= len0)
                  (prod : production Char)
         : bool.
         Proof.
@@ -48,103 +49,117 @@ Section recursive_descent_parser.
                 (** 0-length production, only accept empty *)
                 beq_nat (length str) 0
               | it::its
-                => let parse_production' := fun str pf => parse_production str pf its in
+                => let parse_production' := fun str len pf => parse_production str len pf its in
                    fold_left
                      orb
                      (map (fun n =>
                              (parse_item
-                                (parse_nonterminal (str := take n str) _)
+                                (parse_nonterminal (take n str) (len := min n len) _)
                                 (take n str)
                                 it)
-                               && parse_production' (drop n str) _)%bool
+                               && parse_production' (drop n str) (len - n) _)%bool
                           (split_string_for_production it its str))
                      false
             end;
-          revert pf; clear -HSLP; intros;
-          abstract (rewrite ?str_le_take, ?str_le_drop; assumption).
+          clear -pf;
+          abstract (try apply Min.min_case_strong; omega).
         Defined.
       End production.
 
       Section productions.
-        Context {str0}
+        Context {len0}
                 (parse_nonterminal
                  : forall (str : String)
-                          (pf : str ≤s str0),
+                          (len : nat)
+                          (pf : len <= len0),
                      String.string -> bool).
 
         (** To parse as a given list of [production]s, we must parse as one of the [production]s. *)
         Definition parse_productions
                    (str : String)
-                   (pf : str ≤s str0)
+                   (len : nat)
+                   (pf : len <= len0)
                    (prods : productions Char)
         : bool
           := fold_right orb
                         false
-                        (map (parse_production parse_nonterminal pf)
+                        (map (parse_production parse_nonterminal str pf)
                              prods).
       End productions.
 
 
       Section nonterminals.
         Section step.
-          Context {str0 valid}
+          Context {len0 valid_len}
                   (parse_nonterminal
-                   : forall (p : String * nonterminals_listT),
-                       prod_relation (ltof _ length) nonterminals_listT_R p (str0, valid)
-                       -> forall str : String,
-                            str ≤s fst p -> String.string -> bool).
+                   : forall (p : nat * nat),
+                       prod_relation lt lt p (len0, valid_len)
+                       -> forall (valid : nonterminals_listT)
+                                 (str : String) (len : nat),
+                            len <= fst p -> String.string -> bool).
 
           Definition parse_nonterminal_step
+                     (valid : nonterminals_listT)
                      (str : String)
-                     (pf : str ≤s str0)
+                     (len : nat)
+                     (pf : len <= len0)
                      (nt : String.string)
           : bool.
           Proof.
             refine
               (parse_productions
                  (sumbool_rect
-                    (fun b => forall (str' : String), str' ≤s (if b then str else str0) -> String.string -> bool)
+                    (fun b => forall (str' : String) (len' : nat), len' <= (if b then len else len0) -> String.string -> bool)
                     (fun _ => (** [str] got smaller, so we reset the valid nonterminals list *)
                        @parse_nonterminal
-                         (str : String, initial_nonterminals_data)
-                         (or_introl _))
+                         (len, nonterminals_length initial_nonterminals_data)
+                         (or_introl _)
+                         initial_nonterminals_data)
                     (fun _ => (** [str] didn't get smaller, so we cache the fact that we've hit this nonterminal already *)
                        sumbool_rect
-                         (fun _ => forall (str' : String), str' ≤s str0 -> String.string -> bool)
-                         (fun _ => (** It was valid, so we can remove it *)
+                         (fun _ => forall (str' : String) (len' : nat), len' <= len0 -> String.string -> bool)
+                         (fun is_valid => (** It was valid, so we can remove it *)
                             @parse_nonterminal
-                              (str0 : String, remove_nonterminal valid nt)
-                              (or_intror (conj eq_refl (remove_nonterminal_dec _ nt _))))
+                              (len0, pred valid_len)
+                              (or_intror (conj eq_refl _))
+                              (remove_nonterminal valid nt))
 
-                         (fun _ _ _ _ => (** oops, we already saw this nonterminal in the past.  ABORT! *)
+                         (fun _ _ _ _ _ => (** oops, we already saw this nonterminal in the past.  ABORT! *)
                             false)
-                         (Sumbool.sumbool_of_bool (is_valid_nonterminal valid nt)))
-                    (lt_dec (length str) (length str0)))
-                 (str := str)
+                         (Sumbool.sumbool_of_bool (negb (EqNat.beq_nat valid_len 0) && is_valid_nonterminal valid nt)))
+                    (lt_dec len len0))
+                 str
+                 (len := len)
                  (sumbool_rect
-                    (fun b => str ≤s (if b then str else str0))
-                    (fun _ => or_intror (reflexivity _))
+                    (fun b => len <= (if b then len else len0))
+                    (fun _ => le_n _)
                     (fun _ => _)
-                    (lt_dec (length str) (length str0)))
+                    (lt_dec len len0))
                  (Lookup G nt));
-            assumption.
+            first [ assumption
+                  | simpl;
+                    generalize (proj1 (proj1 (Bool.andb_true_iff _ _) is_valid));
+                    clear; intro;
+                    abstract (
+                        destruct valid_len; try apply Lt.lt_n_Sn; [];
+                        exfalso; simpl in *; congruence
+                  ) ].
           Defined.
         End step.
 
         Section wf.
           (** TODO: add comment explaining signature *)
           Definition parse_nonterminal_or_abort
-          : forall (p : String * nonterminals_listT)
-                   (str : String),
-              str ≤s fst p
+          : forall (p : nat * nat)
+                   (valid : nonterminals_listT)
+                   (str : String) (len : nat),
+              len <= fst p
               -> String.string
               -> bool
             := @Fix
-                 (String * nonterminals_listT)
+                 (nat * nat)
                  _
-                 (well_founded_prod_relation
-                    (well_founded_ltof _ length)
-                    ntl_wf)
+                 (well_founded_prod_relation lt_wf lt_wf)
                  _
                  (fun sl => @parse_nonterminal_step (fst sl) (snd sl)).
 
@@ -153,8 +168,10 @@ Section recursive_descent_parser.
                      (nt : String.string)
           : bool
             := @parse_nonterminal_or_abort
-                 (str : String, initial_nonterminals_data) str
-                 (or_intror (reflexivity _)) nt.
+                 (length str, nonterminals_length initial_nonterminals_data)
+                 initial_nonterminals_data
+                 str (length str)
+                 (le_n _) nt.
         End wf.
       End nonterminals.
     End parts.
