src/Parsers/CorrectnessBaseTypes.v
@@ -9,31 +9,24 @@ Local Open Scope string_like_scope.
 Section general.
   Context {Char} {HSL : StringLike Char} {G : grammar Char}.
 
-  Class boolean_parser_dataT :=
-    { predata :> parser_computational_predataT;
-      split_string_for_production
-      : item Char -> production Char -> String -> list nat }.
-
-  Global Coercion predata : boolean_parser_dataT >-> parser_computational_predataT.
-
-  Definition split_list_completeT `{data : @parser_computational_predataT}
-             {str0 valid}
+  Definition split_list_completeT {data : @parser_computational_predataT}
+             {len0 valid}
              (it : item Char) (its : production Char)
              (str : String)
-             (pf : str ≤s str0)
+             (pf : length str <= len0)
              (split_list : list nat)
 
     := ({ n : nat
-              & (minimal_parse_of_item (G := G) (predata := data) str0 valid (take n str) it)
-                * (minimal_parse_of_production (G := G) str0 valid (drop n str) its) }%type)
+              & (minimal_parse_of_item (G := G) (predata := data) len0 valid (take n str) it)
+                * (minimal_parse_of_production (G := G) len0 valid (drop n str) its) }%type)
        -> ({ n : nat
                  & (In n split_list)
-                   * (minimal_parse_of_item (G := G) str0 valid (take n str) it)
-                   * (minimal_parse_of_production (G := G) str0 valid (drop n str) its) }%type).
+                   * (minimal_parse_of_item (G := G) len0 valid (take n str) it)
+                   * (minimal_parse_of_production (G := G) len0 valid (drop n str) its) }%type).
 
-  Class boolean_parser_completeness_dataT' `{data : boolean_parser_dataT} :=
+  Class boolean_parser_completeness_dataT' {data : boolean_parser_dataT} :=
     { split_string_for_production_complete
-      : forall str0 valid str (pf : str ≤s str0) nt,
+      : forall len0 valid str (pf : length str <= len0) nt,
           is_valid_nonterminal initial_nonterminals_data nt
           -> ForallT
                (Forall_tails
@@ -41,7 +34,7 @@ Section general.
                    => match prod return Type with
                         | nil => True
                         | it::its
-                          => @split_list_completeT data str0 valid it its str pf (split_string_for_production it its str)
+                          => @split_list_completeT data len0 valid it its str pf (split_string_for_production it its str)
                       end))
                (Lookup G nt) }.
 
