src/Parsers/BooleanRecognizerEquality.v
@@ -1,0 +1,132 @@
+(** * The boolean recognizer can work on a projected string type *)
+Require Import ADTSynthesis.Parsers.BooleanRecognizer.
+Require Import ADTSynthesis.Parsers.BaseTypes.
+Require Import ADTSynthesis.Parsers.StringLike.Core.
+Require Import ADTSynthesis.Parsers.ContextFreeGrammarTransfer.
+Require Import ADTSynthesis.Parsers.ContextFreeGrammar.
+Require Import ADTSynthesis.Parsers.BooleanRecognizerCorrect.
+Require Import ADTSynthesis.Common.Wf.
+Require Import ADTSynthesis.Common.SetoidInstances.
+
+Set Implicit Arguments.
+
+Section transfer.
+  Context {Char} {HSL_heavy HSL_lite : StringLike Char} {G : grammar Char}.
+  Context {data : @boolean_parser_dataT Char HSL_heavy}.
+  Context (split_string_for_production_lite
+           : item Char -> production Char -> @String Char HSL_lite -> list nat).
+
+  Class StringLikeProj :=
+    { proj : @String Char HSL_heavy -> @String Char HSL_lite;
+      length_proj : forall str, length (proj str) = length str;
+      drop_proj : forall n str, drop n (proj str) = proj (drop n str);
+      take_proj : forall n str, take n (proj str) = proj (take n str);
+      is_char_proj : forall str ch, is_char (proj str) ch = is_char str ch;
+      split_string_for_production_proj
+      : forall it its str,
+          split_string_for_production_lite it its (proj str)
+          = split_string_for_production it its str }.
+
+  Context {HSLPr : StringLikeProj}.
+
+  Local Instance data' : @boolean_parser_dataT Char HSL_lite
+    := { predata := predata;
+         split_string_for_production it its str
+         := split_string_for_production_lite it its str }.
+
+  Lemma parse_item_proj
+        str_matches_nonterminal str_matches_nonterminal'
+        (H : forall nt, str_matches_nonterminal nt = str_matches_nonterminal' nt)
+        str it
+  : @parse_item _ HSL_lite str_matches_nonterminal (proj str) it
+    = @parse_item _ HSL_heavy str_matches_nonterminal' str it.
+  Proof.
+    unfold parse_item.
+    destruct it.
+    { apply is_char_proj. }
+    { trivial. }
+  Qed.
+
+  Lemma parse_production_proj
+        (len0 : nat)
+        parse_nonterminal parse_nonterminal'
+        (H : forall str len pf' nt,
+               parse_nonterminal (proj str) len pf' nt
+               = parse_nonterminal' str len pf' nt)
+        str len pf prod
+  : @parse_production _ HSL_lite _ len0 parse_nonterminal (proj str) len pf prod
+    = @parse_production _ HSL_heavy _ len0 parse_nonterminal' str len pf prod.
+  Proof.
+    revert len str pf; induction prod; simpl; intros.
+    { rewrite length_proj; reflexivity. }
+    { f_equal; [].
+      rewrite split_string_for_production_proj.
+      apply map_Proper_eq; trivial; [].
+      intro.
+      rewrite take_proj, drop_proj, IHprod.
+      f_equal; [].
+      apply parse_item_proj; trivial. }
+  Qed.
+
+  Lemma parse_productions_proj
+        (len0 : nat)
+        parse_nonterminal parse_nonterminal'
+        (H : forall str len pf' nt,
+               parse_nonterminal (proj str) len pf' nt
+               = parse_nonterminal' str len pf' nt)
+        str len pf prods
+  : @parse_productions _ HSL_lite _ len0 parse_nonterminal (proj str) len pf prods
+    = @parse_productions _ HSL_heavy _ len0 parse_nonterminal' str len pf prods.
+  Proof.
+    unfold parse_productions.
+    f_equal; [].
+    apply map_Proper_eq; trivial; [].
+    intro.
+    apply parse_production_proj; trivial.
+  Qed.
+
+  Lemma parse_nonterminal_step_proj
+        (len0 valid_len : nat)
+        parse_nonterminal parse_nonterminal'
+        (H : forall p pf valid str len pf' nt,
+               parse_nonterminal p pf valid (proj str) len pf' nt
+               = parse_nonterminal' p pf valid str len pf' nt)
+        valid str len pf nt
+  : @parse_nonterminal_step _ HSL_lite G _ len0 valid_len parse_nonterminal valid (proj str) len pf nt
+    = @parse_nonterminal_step _ HSL_heavy G _ len0 valid_len parse_nonterminal' valid str len pf nt.
+  Proof.
+    unfold parse_nonterminal_step.
+    unfold sumbool_rect; simpl.
+    repeat match goal with
+             | [ |- appcontext[match ?e with _ => _ end] ]
+               => destruct e eqn:?
+             | _ => solve [ apply parse_productions_proj; trivial ]
+           end.
+  Qed.
+
+  Lemma parse_nonterminal_or_abort_proj
+        (p : nat * nat) (valid : nonterminals_listT)
+        (str : @String Char HSL_heavy) (len : nat) (pf : len <= fst p) (nt : String.string)
+  : @parse_nonterminal_or_abort _ HSL_lite G _ p valid (proj str) len pf nt
+    = @parse_nonterminal_or_abort _ HSL_heavy G _ p valid str len pf nt.
+  Proof.
+    unfold parse_nonterminal_or_abort.
+    revert valid str len pf nt.
+    match goal with
+      | [ |- appcontext[Fix ?wf _ _ ?a] ]
+        => induction (wf a); intros
+    end.
+    rewrite !Fix5_eq;
+      solve [ apply parse_nonterminal_step_proj; trivial
+            | intros; apply parse_nonterminal_step_ext; trivial ].
+  Qed.
+
+  Lemma parse_nonterminal_proj
+        (str : @String Char HSL_heavy) (nt : String.string)
+  : parse_nonterminal (G := G) (proj str) nt = parse_nonterminal (G := G) str nt.
+  Proof.
+    unfold parse_nonterminal.
+    rewrite length_proj.
+    apply parse_nonterminal_or_abort_proj.
+  Qed.
+End transfer.
