src/Parsers/BooleanRecognizerOptimized.v
@@ -3,7 +3,7 @@ Require Import Coq.Lists.List Coq.Strings.String.
 Require Import Coq.Numbers.Natural.Peano.NPeano Coq.Arith.Compare_dec Coq.Arith.Wf_nat.
 Require Import ADTSynthesis.Parsers.ContextFreeGrammar.
 Require Import ADTSynthesis.Parsers.ContextFreeGrammarNotations.
-Require Import ADTSynthesis.Parsers.BaseTypes ADTSynthesis.Parsers.BooleanBaseTypes.
+Require Import ADTSynthesis.Parsers.BaseTypes.
 Require Import ADTSynthesis.Parsers.StringLike.Properties.
 Require Import ADTSynthesis.Common ADTSynthesis.Common.Wf.
 Require Import ADTSynthesis.Parsers.BooleanRecognizer.
@@ -19,17 +19,17 @@ Global Arguments string_dec : simpl never.
 Global Arguments string_beq : simpl never.
 Global Arguments parse_production _ _ _ _ _ _ _ _ !_.
 
-Lemma parse_production_respectful {Char HSL HSLP predata A B}
-      {f g : forall (a : _ * A) (b : B a) (str : @String Char HSL), str ≤s (fst a) -> String.string -> bool}
-      (H : forall a b c d e, f a b c d e = g a b c d e)
-      str0 a b str pf
+Lemma parse_production_respectful {Char HSL predata A B C}
+      {f g : forall (a : _ * A) (b : B a) (c : C a b) (str : @String Char HSL) (len : nat), len <= (fst a) -> String.string -> bool}
+      (H : forall a b c d e h i, f a b c d e h i = g a b c d e h i)
+      str0 a b c str len pf
 : pointwise_relation
     _ eq
-    (@parse_production Char HSL HSLP predata str0 (f (str0, a) b) str pf)
-    (@parse_production Char HSL HSLP predata str0 (g (str0, a) b) str pf).
+    (@parse_production Char HSL predata str0 (f (str0, a) b c) str len pf)
+    (@parse_production Char HSL predata str0 (g (str0, a) b c) str len pf).
 Proof.
   intro ls.
-  revert str0 a b str pf; induction ls; simpl; trivial; intros.
+  revert str0 a b c str len pf; induction ls; simpl; trivial; intros.
   setoid_rewrite IHls.
   f_equal.
   apply map_Proper_eq; trivial; repeat intro.
@@ -45,7 +45,7 @@ Local Ltac simpl_setoid_rewrite lem :=
     clear H.
 
 Section recursive_descent_parser.
-  Context {Char} {HSL : StringLike Char} {HSLP : StringLikeProperties Char}
+  Context {Char} {HSL : StringLike Char}
           {ls : list (String.string * productions Char)}.
   Context {data : @boolean_parser_dataT Char _}.
   Local Notation G := (list_to_grammar (nil::nil) ls) (only parsing).
@@ -57,64 +57,65 @@ Section recursive_descent_parser.
   Proof.
     let G := match goal with |- context[_ = parse_nonterminal (G := ?G) _ _] => constr:G end in
     let G' := head G in
-    try unfold G';
-      cbv beta iota zeta delta [parse_nonterminal parse_nonterminal_or_abort parse_nonterminal_step parse_productions parse_item Lookup list_to_grammar list_to_productions];
+    try unfold G'.
+    cbv beta iota zeta delta [parse_nonterminal parse_nonterminal_or_abort parse_nonterminal_step parse_productions parse_item Lookup list_to_grammar list_to_productions].
+    simpl.
+    eexists.
+    let L := match goal with |- ?L = _ => constr:L end in
+    let e := fresh "e" in
+    let e' := fresh "e" in
+    let pp := fresh "pp" in
+    set (e := L);
+      etransitivity;
+      [
+      | match goal with
+          | [ |- _ = @Fix ?A ?R ?Rwf (fun a : ?A => forall (b :@?B a) (c : @?C a b) (d : @?D a b c) (e : @?E a b c d) (h : @?H a b c d e), @?P a b c d e h) ?f ?a ?b ?c ?d ?e ?h ]
+            => refine ((fun H0 => @Fix5_Proper_eq A B C D E H R Rwf P _ f H0 a b c d e h) _)
+        end;
+        unfold forall_relation, pointwise_relation, respectful;
+        let H' := fresh in
+        (intros ??? H' ?????);
+          let L := match goal with |- ?L = ?R => constr:L end in
+          let R := match goal with |- ?L = ?R => constr:R end in
+          set (e' := L);
+            let R' := match type of H' with
+                        | forall a0 a1 a2 a3 a4 a5 a6, ?x a0 a1 a2 a3 a4 a5 a6 = ?y a0 a1 a2 a3 a4 a5 a6
+                          => let Rp := (eval pattern y in R) in
+                             match Rp with
+                               | ?R' y => (eval cbv beta in (R' x))
+                             end
+                      end in
+            transitivity R';
+              [ clear H';
+                match goal with
+                  | [ |- appcontext[@parse_production ?a ?b ?c ?d ?e ?f ?g ?h] ]
+                    => set (pp := @parse_production a b c d e f g h)
+                end
+              | clear -H'; unfold sumbool_rect;
+                repeat match goal with
+                         | _ => reflexivity
+                         | [ |- appcontext[match ?e with left _ => _ | right _ => _ end] ]
+                           => destruct e
+                       end;
+                setoid_rewrite (parse_production_respectful H');
+                reflexivity ] ];
+      [
+      | repeat match goal with
+                 | _ => progress simpl
+                 | _ => setoid_rewrite (fun ls => eq_sym (@fold_symmetric _ orb Bool.orb_assoc Bool.orb_comm false ls))
+                 | _ => setoid_rewrite Bool.orb_false_r
+                 | [ |- appcontext[fold_right (fun str_t else_case s => bool_rect (fun _ => ?T) (@?a str_t) (else_case s) (@?b str_t s))] ]
+                   => simpl_setoid_rewrite (@fold_right_fun _ _ _ (fun str_t else_cases s => bool_rect (fun _ => T) (a str_t) else_cases (b str_t s)))
+                 | [ |- appcontext[?f (fold_right (fun x acc => bool_rect (fun _ => _) _ acc _) _ ?ls) ?x] ]
+                   => simpl_setoid_rewrite (fun init => @f_fold_right_bool_rect _ _ _ (fun k => f k x) init ls)
+                 | [ |- appcontext[?f (fold_right (fun x acc => bool_rect (fun _ => _) _ acc _) _ ?ls)] ]
+                   => simpl_setoid_rewrite (fun init => @f_fold_right_bool_rect _ _ _ f init ls)
+               end;
+        subst pp; simpl;
+        subst e'; instantiate; reflexivity ];
+      cbv beta iota zeta delta [bool_rect sumbool_rect];
       simpl;
-      eexists;
-      let L := match goal with |- ?L = _ => constr:L end in
-      let e := fresh "e" in
-      let e' := fresh "e" in
-      let pp := fresh "pp" in
-      set (e := L);
-        etransitivity;
-        [
-        | match goal with
-            | [ |- _ = @Fix ?A ?R ?Rwf (fun a : ?A => forall (b :@?B a) (c : @?C a b) (d : @?D a b c), @?P a b c d) ?f ?a ?b ?c ?d ]
-              => refine ((fun H => @Fix3_Proper_eq A B C D R Rwf P _ f H a b c d) _)
-          end;
-          unfold forall_relation, pointwise_relation, respectful;
-          let H' := fresh in
-          (intros ??? H' ???);
-            let L := match goal with |- ?L = ?R => constr:L end in
-            let R := match goal with |- ?L = ?R => constr:R end in
-            set (e' := L);
-              let R' := match type of H' with
-                          | forall a0 a1 a2 a3 a4, ?x a0 a1 a2 a3 a4 = ?y a0 a1 a2 a3 a4
-                            => let Rp := (eval pattern y in R) in
-                               match Rp with
-                                 | ?R' y => (eval cbv beta in (R' x))
-                               end
-                        end in
-              transitivity R';
-                [ clear H';
-                  match goal with
-                    | [ |- appcontext[@parse_production ?a ?b ?c ?d ?e ?f ?g ?h] ]
-                      => set (pp := @parse_production a b c d e f g h)
-                  end
-                | clear -H'; unfold sumbool_rect;
-                  repeat match goal with
-                           | _ => reflexivity
-                           | [ |- appcontext[match ?e with left _ => _ | right _ => _ end] ]
-                             => destruct e
-                         end;
-                  setoid_rewrite (parse_production_respectful H');
-                  reflexivity ] ];
-        [
-        | repeat match goal with
-                   | _ => progress simpl
-                   | _ => setoid_rewrite (fun ls => eq_sym (@fold_symmetric _ orb Bool.orb_assoc Bool.orb_comm false ls))
-                   | _ => setoid_rewrite Bool.orb_false_r
-                   | [ |- appcontext[fold_right (fun str_t else_case s => bool_rect (fun _ => ?T) (@?a str_t) (else_case s) (@?b str_t s))] ]
-                     => simpl_setoid_rewrite (@fold_right_fun _ _ _ (fun str_t else_cases s => bool_rect (fun _ => T) (a str_t) else_cases (b str_t s)))
-                   | [ |- appcontext[?f (fold_right (fun x acc => bool_rect (fun _ => _) _ acc _) _ ?ls) ?x] ]
-                     => simpl_setoid_rewrite (fun init => @f_fold_right_bool_rect _ _ _ (fun k => f k x) init ls)
-                   | [ |- appcontext[?f (fold_right (fun x acc => bool_rect (fun _ => _) _ acc _) _ ?ls)] ]
-                     => simpl_setoid_rewrite (fun init => @f_fold_right_bool_rect _ _ _ f init ls)
-                 end;
-          subst pp; simpl;
-          subst e'; instantiate; reflexivity ];
-        cbv beta iota zeta delta [bool_rect sumbool_rect];
-        subst e; instantiate.
+      subst e; instantiate.
     reflexivity.
   Defined.
 End recursive_descent_parser.
