src/Parsers/ParserImplementationOptimized.v
@@ -1,7 +1,8 @@
 (** * Implementation of simply-typed interface of the parser *)
 Require Export ADTSynthesis.Parsers.ParserInterface.
-Require Import ADTSynthesis.Parsers.BaseTypes ADTSynthesis.Parsers.BooleanBaseTypes.
+Require Import ADTSynthesis.Parsers.BaseTypes ADTSynthesis.Parsers.CorrectnessBaseTypes.
 Require Import ADTSynthesis.Parsers.BooleanRecognizerOptimized.
+Require Import ADTSynthesis.Parsers.BooleanRecognizerEquality.
 Require Import ADTSynthesis.Parsers.ParserImplementation.
 Require Import ADTSynthesis.Parsers.ContextFreeGrammarNotations.
 Require Import ADTSynthesis.Parsers.ContextFreeGrammarTransfer.
@@ -62,19 +63,34 @@ Section implementation.
   Context {ls : list (String.string * productions Ascii.ascii)}.
   Local Notation G := (list_to_grammar (nil::nil) ls) (only parsing).
   Context (splitter : Splitter G).
+  Context {string_like_lite : StringLike Ascii.ascii}
+          split_string_for_production_lite
+          (HSLPr : @StringLikeProj Ascii.ascii splitter string_like_lite (parser_data splitter) split_string_for_production_lite).
   Context (make_string : String.string -> @String _ splitter)
           (R : @String _ splitter -> @String _ string_stringlike -> Prop)
           (R_make : forall str, R (make_string str) str)
           (R_respectful : transfer_respectful R)
           (R_flip_respectful : transfer_respectful (Basics.flip R)).
 
-  Local Instance parser_data : @boolean_parser_dataT Ascii.ascii splitter := parser_data splitter.
+  Local Instance pdata : @boolean_parser_dataT Ascii.ascii string_like_lite
+    := @data' _ splitter string_like_lite (parser_data splitter) split_string_for_production_lite.
+  Local Instance pdata' : @boolean_parser_dataT Ascii.ascii splitter
+    := parser_data splitter.
 
   Definition parser : Parser G string_stringlike.
   Proof.
-    let impl := (eval simpl in (fun str => proj1_sig (parse_nonterminal_opt (ls := ls) (data := parser_data) (make_string str) (Start_symbol G)))) in
+    let impl0 := constr:(fun str => (parse_nonterminal_opt (ls := ls) (data := pdata) (proj (make_string str)) (Start_symbol G))) in
+    let impl := (eval simpl in (fun str => proj1_sig (impl0 str))) in
+    let implH := constr:(fun str => proj2_sig (impl0 str)) in
     let impl' := (eval cbv beta iota zeta delta [RDPList.rdp_list_remove_nonterminal RDPList.rdp_list_nonterminals_listT RDPList.rdp_list_is_valid_nonterminal RDPList.rdp_list_ntl_wf RDPList.rdp_list_nonterminals_listT_R] in impl) in
     let impl := (eval simpl in impl') in
-    refine (transfer_parser (parser splitter) make_string impl (fun str => proj2_sig (parse_nonterminal_opt (ls := ls) (data := parser_data) (make_string str) (Start_symbol G))) R R_make _ _).
+    refine (transfer_parser
+              (HSL1 := splitter) (HSL2 := string_stringlike)
+              (parser splitter) make_string
+              impl
+              (fun str => eq_trans
+                            (implH str)
+                            (@parse_nonterminal_proj _ splitter string_like_lite G pdata' _ HSLPr _ _))
+              R R_make _ _).
   Defined.
 End implementation.
