src/Parsers/Refinement/SharpenedExpressionParen.v
@@ -47,89 +47,11 @@ Global Arguments ComputationalSplitter / .
 
 Require Import ADTSynthesis.Parsers.ParserFromParserADT.
 Require Import ADTSynthesis.Parsers.ExtrOcamlParsers.
-(*
-Ltac do_simpl_in x hyp :=
-  let x' := (eval simpl in x) in
-  change x with x' in hyp.
-Ltac do_compute_in x hyp :=
-  let x' := (eval compute in x) in
-  change x with x' in hyp.
+Import ADTSynthesis.Parsers.ExtrOcamlParsers.HideProofs.
 
-Definition paren_expr_parser (str : String.string) : bool.
-Proof.
-  pose (has_parse (parser ComputationalSplitter) str) as impl.
-  Timeout 60 cbv beta iota zeta delta [has_parse parser ParserImplementationOptimized.parser transfer_parser prod_relation ltof list_to_productions new_string_of_string new_string_of_base_string item_ascii_cons item_ascii item_of_char item_of_string BooleanRecognizer.parse_production BooleanRecognizer.parse_item ComputationalSplitter BooleanBaseTypes.split_string_for_production If_Then_Else fst snd projT1 projT2 ContextFreeGrammarEquality.production_beq Equality.list_beq ContextFreeGrammarEquality.item_beq Equality.ascii_beq StringBound.bindex StringBound.indexb ComputationalADT.cConstructors Equality.bool_beq map hd fold_left fold_right list_to_grammar Start_symbol Lookup bool_rect StringLike.String item_ascii_cons item_ascii item_of_char item_of_string new_string_of_base_string BooleanRecognizer.parse_production BooleanRecognizer.parse_item BooleanBaseTypes.split_string_for_production ParserImplementation.parser is_char StringLike.length string_stringlike BooleanRecognizerOptimized.parse_nonterminal_opt proj1_sig proj2_sig ComputationalADT.cADT string_rep ComputationalADT.LiftcADT SplitterFromParserADT.adt_based_splitter orb andb] in impl.
-
-Print CallConstructor.
-Locate "=p".
-  Timeout 2 simpl is_char in impl.
-  Timeout 2 simpl ((CallConstructor (projT1 ComputationalSplitter) "new")) in impl.
-  Timeout 2 cbv beta iota zeta in impl.
-  Timeout 15 simpl (BooleanBaseTypes.split_string_for_production _ _) in impl.
-  Timeout 5 cbv beta iota zeta in impl.
-  Timeout 2 simpl hd in impl.
-  Timeout 2 simpl (map fst _) in impl.
-  Timeout 2 cbv beta iota zeta delta [map] in impl.
-  Timeout 2 change (fst (?x, _)) with x in impl.
-  Timeout 2 change (snd (_, ?x)) with x in impl.
-  Timeout 2 cbv beta iota zeta delta [hd] in impl.
-  Timeout 2 cbv beta iota zeta delta [fold_left] in impl.
-  Timeout 2 change (fst (?x, _)) with x in impl.
-  Timeout 2 change (snd (_, ?x)) with x in impl.
-  Timeout 2 cbv beta iota zeta delta [fold_right] in impl.
-  Timeout 5 change (fst (?x, _)) with x in impl.
-  Timeout 5 change (snd (_, ?x)) with x in impl.
-  Timeout 5 cbv beta iota zeta in impl.
-  Timeout 5 cbv beta iota zeta delta [] in impl.
-  Timeout 10 change (orb false) with (fun x : bool => x) in impl.
-  Timeout 2 cbv beta iota zeta delta [new_string_of_base_string] in impl.
-  Timeout 2 cbv beta iota zeta delta [] in impl.
-  Timeout 2 cbv beta iota zeta delta [item_ascii_cons item_ascii item_of_char item_of_string] in impl.
-  Timeout 10 cbv beta iota zeta delta [BooleanRecognizer.parse_production] in impl.
-  Timeout 10 cbv beta iota zeta delta [BooleanRecognizer.parse_item] in impl.
-
-  Timeout 5 lazymatch eval cbv delta [impl] in impl with
-    | appcontext [@BooleanBaseTypes.split_string_for_production
-                 ?a ?b ?c ?d ?e]
-      => set (X := @BooleanBaseTypes.split_string_for_production
-                     a b c d e)
-  end.
-                           (Terminal "1"%char) [])).
-  Timeout 25 simpl (BooleanBaseTypes.split_string_for_production _) in impl.
-  Timeout 10 cbv beta iota zeta delta [] in impl.
-  Timeout 5 cbv beta iota zeta delta [map] in impl.
-  Timeout 10 cbv beta iota zeta delta [fold_left] in impl.
-  Timeout 10 cbv beta iota zeta delta [fold_left] in impl.
-
-
-  Timeout 2 change (fst (?x, _)) with x in impl.
-  Timeout 2 change (snd (_, ?x)) with x in impl.
-  Timeout 2 cbv beta iota zeta delta [fold_right] in impl.
-  Timeout 2 change (fst (?x, _)) with x in impl.
-  Timeout 5 change (snd (_, ?x)) with x in impl.
-
-
-  Unset Printing Notations.
- := item Ascii.ascii.
-Coercion item_of_char (ch : Ascii.ascii) : item_ascii := Terminal ch.
-Coercion item_of_string (nt : string) : item_ascii := NonTerminal nt.
-Definition production_of_string] in impl.
-
-  Timeout 2 simpl fst in impl.
-
-Timeout 2 simpl @list_to_grammar in impl.
-  Timeout 2 simpl @list_to_productions in impl.
-
-  Timeout 10 simpl map in impl.
-
-
-  Timeout 2 cbv beta iota zeta delta [has_parse] in impl.
-*)
 Time Definition paren_expr_parser (str : String.string) : bool
   := Eval simpl in has_parse (parser ComputationalSplitter) str.
 
-Print paren_expr_parser.
-Import ADTSynthesis.Parsers.ExtrOcamlParsers.HideProofs.
 Print paren_expr_parser.
 
 Recursive Extraction paren_expr_parser.
