src/Parsers/Splitters/Reflective.v
@@ -1,7 +1,7 @@
 (** * Reflective lemmas for proving a splitter complete *)
 Require Import Coq.Lists.List Coq.Strings.String.
 Require Import ADTSynthesis.Parsers.ContextFreeGrammar.
-Require Import ADTSynthesis.Parsers.BaseTypes ADTSynthesis.Parsers.BooleanBaseTypes.
+Require Import ADTSynthesis.Parsers.BaseTypes ADTSynthesis.Parsers.CorrectnessBaseTypes.
 Require Import ADTSynthesis.Parsers.Splitters.RDPList.
 Require Import Coq.Init.Wf.
 Require Import Coq.Arith.Wf_nat.
